factor out a module for ghost fractional tables

pulse/lib/pulse/lib/Pulse.Lib.SLPropTable.fst
@@ -1,49 +1,23 @@
 module Pulse.Lib.SLPropTable
 #lang-pulse
 open Pulse.Lib.Pervasives
-module PM = Pulse.Lib.PCMMap
-module PF = Pulse.Lib.PCM.Fraction
-module GR = Pulse.Lib.GhostReference
-module GPR = Pulse.Lib.GhostPCMReference
-let slprop_map = PM.pointwise nat (PF.pcm_frac #really_big_ref)
-let carrier = PM.map nat (PF.fractional really_big_ref)
-let tab = GPR.gref slprop_map
+module GT = Pulse.Lib.GhostFractionalTable
+let table = GT.table really_big_ref
 
-[@@erasable]
-let table = erased tab
+instance non_informative_table
+: NonInformative.non_informative table
+= _ by (FStar.Tactics.Typeclasses.tcresolve())
 
-instance non_informative_table: NonInformative.non_informative table = {
-  reveal = (fun (x:erased table) -> FStar.Ghost.reveal x)
-}
-
-let full_perm : perm = 1.0R
-let full_table_above (n:nat) (r:really_big_ref)
-: carrier
-= Map.map_literal 
-  (fun (k:nat) -> 
-    if k < n
-    then None
-    else Some (r, full_perm))
-
-let singleton (i:nat) (f:perm) (r:really_big_ref) 
-: carrier
-= Map.map_literal
-  (fun (k:nat) -> 
-    if k = i
-    then Some (r, f)
-    else None)
-
+[@@pulse_unfold]
 let is_table (t:table) (max:nat)
 : slprop
-= exists* default_r.
-    GPR.pts_to t (full_table_above max default_r)
+= GT.is_table t max
 
 let pts_to (t:table) (i:nat) (#f:perm) (p:slprop)
 : slprop
 = exists* r.
     really_big_pts_to r p **
-    GPR.pts_to t (singleton i f r) **
-    pure (PF.perm_ok f)
+    GT.pts_to t i #f r
 
 ghost
 fn create ()
@@ -51,84 +25,8 @@ requires emp
 returns t:table
 ensures is_table t 0
 {
-  // let max : GR.ref nat = GR.alloc #nat 0;
-  let default_r = really_big_alloc emp;
-  drop_ (really_big_pts_to _ _);
-  let gref = GPR.alloc #_ #slprop_map (full_table_above 0 default_r);
-  fold (is_table gref 0);
-  gref
-}
-
-let fp_upd_singleton (i:nat) (r0 r1:really_big_ref)
-: FStar.PCM.frame_preserving_upd
-    slprop_map
-    (singleton i full_perm r0)
-    (singleton i full_perm r1)
-= let fp = PF.mk_frame_preserving_upd r0 r1 in
-  let fp = PM.lift_frame_preserving_upd _ _ fp (singleton i full_perm r0) i in
-  assert (
-    Map.equal (singleton i full_perm r1)
-              (Map.upd (singleton i full_perm r0) i (Some (r1, full_perm)))
-  );
-  fp
-
-ghost
-fn update_i (r:GPR.gref slprop_map) (i:nat) (f:perm) (r0 r1: really_big_ref)
-requires 
-  GPR.pts_to r (singleton i full_perm r0)
-ensures
-  GPR.pts_to r (singleton i full_perm r1)
-{
-  GPR.write r _ _ (fp_upd_singleton i r0 r1);
-}
-
-ghost
-fn share_i (r:GPR.gref slprop_map) (i:nat) (f0 f1:perm) (v: really_big_ref)
-requires 
-  GPR.pts_to r (singleton i (f0 +. f1) v) ** pure (PF.perm_ok (f0 +. f1))
-ensures
-  GPR.pts_to r (singleton i f0 v) **
-  GPR.pts_to r (singleton i f1 v)
-{
-  assert pure (
-    Map.equal 
-      (singleton i (f0 +. f1) v)
-      (singleton i f0 v `FStar.PCM.op slprop_map` singleton i f1 v)
-  );
-  GPR.share r (singleton i f0 v) (singleton i f1 v)
-}
-
-ghost
-fn gather_i (r:GPR.gref slprop_map) (i:nat) (f0 f1:perm) (v0 v1: really_big_ref)
-requires 
-  GPR.pts_to r (singleton i f0 v0) **
-  GPR.pts_to r (singleton i f1 v1)
-ensures
-  GPR.pts_to r (singleton i (f0 +. f1) v0) **
-  pure (v0 == v1 /\ PF.perm_ok (f0 +. f1))
-{
-  GPR.gather r (singleton i f0 v0) (singleton i f1 v1);
-  assert pure (
-    Map.equal 
-      (singleton i (f0 +. f1) v0)
-      (singleton i f0 v0 `FStar.PCM.op slprop_map` singleton i f1 v1)
-  )
-}
-
-ghost
-fn take_i (r:GPR.gref slprop_map) (n:nat) (#dr:_)
-requires 
-  GPR.pts_to r (full_table_above n dr)
-ensures
-  GPR.pts_to r (full_table_above (n + 1) dr) **
-  GPR.pts_to r (singleton n full_perm dr)
-{
-  assert pure (
-    Map.equal 
-      (full_table_above n dr)
-      (full_table_above (n + 1) dr `FStar.PCM.op slprop_map` singleton n full_perm dr)
-  );
-  GPR.share r (full_table_above (n + 1) dr) (singleton n full_perm dr)
+  let t = GT.create #really_big_ref;
+  t
 }
 
 ghost
@@ -144,7 +42,7 @@ ensures
   unfold pts_to;
   drop_ (really_big_pts_to _ _);
   let r' = really_big_alloc p;
-  update_i t i full_perm _ r';
+  GT.update t r';
   fold pts_to
 }
 
@@ -156,12 +54,9 @@ ensures
   is_table t (i + 1) **
   pts_to t i #1.0R p
 {
-  unfold is_table;
-  take_i t i;
   let r = really_big_alloc p;
-  update_i t i full_perm _ r;
+  GT.alloc t r;
   fold pts_to;
-  fold is_table;
 }
 
 
@@ -172,13 +67,9 @@ requires
 ensures
   is_table t n ** pts_to t i #f p ** pure (i < n)
 {
-  if (i >= n) 
-  {
-    unfold is_table;
-    unfold pts_to;
-    GPR.gather t _ _;
-    unreachable()
-  }
+  unfold pts_to;
+  GT.in_bounds t;
+  fold pts_to;
 }
 
 ghost
@@ -189,8 +80,7 @@ ensures
   pts_to t i #f0 p ** pts_to t i #f1 p
 {
   unfold pts_to;
-  with r. assert (GPR.pts_to t (singleton i f r));
-  share_i t i f0 f1 r;
+  GT.share t i f0 f1;
   really_big_share _;
   fold (pts_to t i #f0 p);
   fold pts_to;
@@ -204,10 +94,10 @@ ensures
    pts_to t i #(f0 +. f1) p ** later (equiv p q)
 {
   unfold (pts_to t i #f0 p);
-  with r0. assert (GPR.pts_to t (singleton i f0 r0));
+  with r0. assert (GT.pts_to t i #f0 r0);
   unfold pts_to;
-  with r1. assert (GPR.pts_to t (singleton i f1 r1));
-  gather_i t i f0 f1 r0 r1;
+  with r1. assert (GT.pts_to t i #f1 r1);
+  GT.gather t i #f0 #f1 #r0 #r1;
   really_big_gather r0 #p #q;
   fold (pts_to t i #(f0 +. f1) p);
 }
